---
title: "Math Refresher: Basic Calculus"
format: html
---

## Introduction

This is a refresher on basic calculus.  It is not meant to be a substitute for a full course on calculus, but rather a quick review of the basic concepts and techniques that will be used in this semester.  

## Limits

The limit of a function $f(x)$ as $x$ approaches $a$ is the value that $f(x)$ approaches as $x$ gets closer and closer to $a$.  We write this as:

$$\lim_{x \to a} f(x) = L$$

In this case, the limit of the function $f(x)$ as $x$ approaches $a$ is $L$.  For example, consider the function $f(x) = x^2$.  The limit of $f(x)$ as $x$ approaches $2$ is $4$:

## Limits to Derivatives

Limits can also be used to estimate derivatives. The derivative of a function $f(x)$ is the slope of the function at a given point.  The derivative of $f(x)$ at $x = a$ is written as $f'(a)$.  The derivative of $f(x)$ is defined as:

$$f'(a) = \lim_{h \to 0} \frac{f(a+h) - f(a)}{h}$$

In other words, the deriviative is the slope of a function at a particular point $a$. This can be proxied using derivatives, by choosing a very small value for $h$.  

For example, consider the function $f(x) = x^2$.  The derivative of $f(x)$ at $x = a$ is:

$$\begin{aligned}
f'(a) &= \lim_{h \to 0} \frac{f(a+h) - f(a)}{h} \\
&=\lim_{h \to 0} \frac{(a+h)^2 - (a)^2}{h} \\
&= \lim_{h \to 0} \frac{a^2 + 2ah + h^2 - a^2}{h} \\
&= \lim_{h \to 0} 2a + h= 2a
\end{aligned}
$$

If anything else fails, one can always rely on numerical differentiation.  

## Derivative of common functions

For most common functions, the derivative can be calculated using the following rules:

- The derivative of a constant is zero
- The derivative of $x^n$ is $nx^{n-1}$
- The derivative of $ln(x)$ is $\frac{1}{x}$
- The derivative of $e^x$ is $e^x$
- The derivative of $a^x$ is $a^x \ln a$

There are other rules for derivatives, but these are the ones that will be used most often.

## Derivative of composite functions

The derivative of a composite function $f(g(x))$ is given by the chain rule:

$$\frac{d}{dx} f(g(x)) = f'(g(x)) g'(x)$$

For example, consider the function $f(x) = \ln(x^2)$.  The derivative of $f(x)$ is:

$$\begin{aligned}
\frac{d}{dx} \ln(x^2) &= \frac{1}{x^2} \frac{d}{dx} x^2 \\
&= \frac{1}{x^2} 2x \\
&= \frac{2}{x}
\end{aligned}
$$

## Derivative of sums and products

The derivative of a sum of functions is the sum of the derivatives of the functions. 

$$\frac{d}{dx} (f(x) + g(x)) = \frac{d}{dx} f(x) + \frac{d}{dx} g(x)$$

The derivative of a product of functions is given by the product rule:

$$\frac{d}{dx} (f(x) g(x)) = f'(x) g(x) + f(x) g'(x)$$

The derivative of a quotient of functions is given by the quotient rule:

$$\frac{d}{dx} \frac{f(x)}{g(x)} = \frac{f'(x) g(x) - f(x) g'(x)}{g(x)^2}$$

Which is a special case of th product rule.

# Maximization and Minimization

Derivatives can be used to identify the maximum and minimum values of a function. Consider a function $f(x)$. 

To find the maximum (or minimum) value of $f(x)$, we can take the derivative of $f(x)$ and set it equal to zero. 
This is called the first order condition. The idea is that at the maximum (or minimum) value of $f(x)$ shouldnt change anymore (should be flat). Thus the derivative of $f(x)$ should be zero.

For example, consider the function $f(x) = 5x^2 - 4 x + 2$.  The derivative of $f(x)$ is:

$$\begin{aligned}
f'(x) &= 10x - 4 =0 \\
x &= \frac{4}{10} = 0.4
\end{aligned}
$$

So when $x$ is equal to $0.4$, the function $f(x)$ does not change anymore. This, however, is insufficient to determine if the function is at a maximum or a minimum.  To determine this, we can take the second derivative of $f(x)$, or second order condition:

$$\begin{aligned}
f''(x) &= 10 > 0
\end{aligned}
$$

Because the second derivative is positive, we know that $f(x)$ is at a minimum when $x = 0.4$.  If the second derivative was negative, we would know that $f(x)$ is at a maximum when $x = 0.4$.

why is this the case

- $f'(x)$ measures the changes in $f(x)$ along x. when $f'(x) = 0$, $f(x)$ is not changing anymore.
- $f''(x)$ measures the changes in $f'(x)$ (changes in those changes). Because its positive, we know that $f'(x)$ is increasing. This means that at $x=0.4$ the changes if $f(x)$ were going from negative to positive. Thus indicating a minimum.

## Optimization with multiple variables

When considering multiple variables, we also need to rely on the first and second order conditions to find minimum and maximum values.  Consider a function $f(x,y)$.  The first order conditions are:

$$\begin{aligned}
\frac{\partial}{\partial x} f(x,y) &= 0 \\
\frac{\partial}{\partial y} f(x,y) &= 0
\end{aligned}
$$

This conditions now say that, in the direction of $x$ and $y$, the function $f(x,y)$ is not changing anymore. Thus we have a potential maximum or minimum. Now, to identify a minimum, we need second order conditions to be:

$$\begin{aligned}
H=\begin{bmatrix}
f_{xx} & f_{xy} \\
f_{xy} & f_{yy} \\
\end{bmatrix}
\end{aligned}
$$

If $Det(H)>0$ and $f_{xx}>0$ then we have a minimum. If $Det(H)>0$ and $f_{xx}<0$ then we have a maximum. If $Det(H)<0$ then we have a saddle point. And if $Det(H)=0$ then we have an inconclusive result.

## Optimization with constraints

When optimizing a function with constraints, we can use the method of Lagrange multipliers.  Consider a function $f(x,y)$ subject to the constraint $g(x,y) = z$.  The Lagrangian is:

$$\begin{aligned}
L(x,y,\lambda) = f(x,y) + \lambda (z - g(x,y))
\end{aligned}
$$

Notice that the Lagrangian is the function $f(x,y)$ plus the constraint $g(x,y)$ multiplied by a constant $\lambda$.  The constant $\lambda$ is called the Lagrange multiplier.  The constrain is written as the difference between the constant $z$ and the function $g(x,y)$.  The Lagrangian is then optimized with respect to $x$, $y$, and $\lambda$. This are the equivalent of the first order conditions:

$$\begin{aligned}
\frac{\partial}{\partial x} L(x,y,\lambda) &= 0 \\
\frac{\partial}{\partial y} L(x,y,\lambda) &= 0 \\
\frac{\partial}{\partial \lambda} L(x,y,\lambda) &= z - g(x,y)=0
\end{aligned}
$$

The last condition is the constraint, and it implies that the constraint must be satisfied.  The second order conditions are the same as before.

